finger-tree: definition and proof of [concat].

finger-tree/FingerTree.v
@@ -13,8 +13,8 @@ Section AbsurdAux.
   Qed.
 
   Lemma absurd5 :
-    forall (A : Type) (a b c d e : A) (l : list A),
-      1 <= length (a :: b :: c :: d :: e :: l) <= 4 -> False.
+    forall (A : Type) (a b c d e : A) (l : list A) (n : nat),
+      n <= length (a :: b :: c :: d :: e :: l) <= 4 -> False.
   Proof.
     simpl; intros; omega.
   Qed.
@@ -35,11 +35,86 @@ Inductive FingerTree (A : Type) : Type :=
 | single : A -> FingerTree A
 | deep : Digit A -> FingerTree (Node A) -> Digit A -> FingerTree A.
 
+Arguments empty {A}.
+
+Definition digitToTree (A : Type) (ds : Digit A) : FingerTree A.
+  refine (
+    match ds with
+    | exist _ [] H => absurd0 H
+    | exist _ [a] _ => single a
+    | exist _ [a; b] _ => deep {[a]} empty {[b]}
+    | exist _ [a; b; c] _ => deep {[a; b]} empty {[c]}
+    | exist _ [a; b; c; d] _ => deep {[a; b]} empty {[c; d]}
+    | exist _ _ H => absurd5 H
+    end
+  ); simpl; intuition.
+Defined.
+
+Definition nodeToList (A : Type) (node : Node A) : list A :=
+  match node with
+  | node2 a b => [a; b]
+  | node3 a b c => [a; b; c]
+  end.
+
+Definition nodeToDigit (A : Type) (node : Node A) : Digit A.
+  refine (
+    match node with
+    | node2 a b => {[a; b]}
+    | node3 a b c => {[a; b; c]}
+    end
+  ); simpl; intuition.
+Defined.
+
+(* [SemiDigit] is similar to [Digit], but allows empty list. *)
+Definition SemiDigit (A : Type) := { l : list A | 0 <= length l <= 4 }.
+
+Definition fromDigit {A : Type} (t : Digit A) : SemiDigit A.
+  refine (match t with exist _ t _ => {t} end);
+  omega.
+Defined.
+
+Fixpoint concatToNodes' {A : Type} (a b : A) (xs : list A) : list (Node A) :=
+  match xs with
+  | [] => [node2 a b]
+  | [c] => [node3 a b c]
+  | [c; d] => [node2 a b; node2 c d]
+  | c :: d :: e :: xs => node3 a b c :: concatToNodes' d e xs
+  end.
+
+Lemma concatToNodes'_length :
+  forall (A : Type) (a b : A) (xs : list A),
+    length xs <= 10 ->
+    1 <= length (concatToNodes' a b xs) <= 4.
+Proof.
+  intros; do 11 (destruct xs; simpl in *; auto; try omega).
+Qed.
+
+Definition concatToNodes {A : Type} (xs : list A)
+                         (H : 2 <= length xs <= 12) : Digit (Node A).
+  destruct xs as [| a]; simpl in *. omega.
+  destruct xs as [| b]; simpl in *. omega.
+  pose (concatToNodes' a b xs).
+  assert (length xs <= 10). omega.
+  assert (1 <= length l <= 4). apply concatToNodes'_length; auto.
+  exact (exist _ l H1).
+Defined.
+
+Definition concatDigits {A : Type} (a : Digit A)
+                                   (b : SemiDigit A)
+                                   (c : Digit A) : Digit (Node A).
+  refine (
+    match a, b, c with
+    | exist _ a _, exist _ b _, exist _ c _ => concatToNodes (a ++ b ++ c) _
+    end
+  ).
+  repeat (rewrite app_length); omega.
+Defined.
+
 Fixpoint cons {A : Type} (a : A) (t : FingerTree A) : FingerTree A.
   refine (
     match t with
-    | empty _ => single a
-    | single b => deep {[a]} (empty _) {[b]}
+    | empty => single a
+    | single b => deep {[a]} empty {[b]}
     | deep l m r =>
         match l with
         | exist _ [] H => absurd0 H
@@ -57,8 +132,8 @@ Defined.
 Fixpoint snoc {A : Type} (a : A) (t : FingerTree A) : FingerTree A.
   refine (
     match t with
-    | empty _ => single a
-    | single b => deep {[b]} (empty _) {[a]}
+    | empty => single a
+    | single b => deep {[b]} empty {[a]}
     | deep l m r =>
         match r with
         | exist _ [] H => absurd0 H
@@ -84,39 +159,18 @@ Inductive ViewR (A : Type) :=
 | emptyR : ViewR A
 | consR : FingerTree A -> A -> ViewR A.
 
-Definition SemiDigit (A : Type) := { l : list A | 0 <= length l <= 3 }.
-
-Definition digitToTree (A : Type) (ds : Digit A) : FingerTree A.
-  refine (
-    match ds with
-    | exist _ [] H => absurd0 H
-    | exist _ [a] _ => single a
-    | exist _ [a; b] _ => deep {[a]} (empty _) {[b]}
-    | exist _ [a; b; c] _ => deep {[a; b]} (empty _) {[c]}
-    | exist _ [a; b; c; d] _ => deep {[a; b]} (empty _) {[c; d]}
-    | exist _ _ H => absurd5 H
-    end
-  ); simpl; intuition.
-Defined.
-
-Definition nodeToDigit (A : Type) (node : Node A) : Digit A.
-  refine (
-    match node with
-    | node2 a b => {[a; b]}
-    | node3 a b c => {[a; b; c]}
-    end
-  ); simpl; intuition.
-Defined.
+Arguments emptyL {A}.
+Arguments emptyR {A}.
 
 Fixpoint viewL {A : Type} (t : FingerTree A) : ViewL A.
   refine (
     match t with
-    | empty _ => emptyL _
-    | single a => consL a (empty _)
+    | empty => emptyL
+    | single a => consL a empty
     | deep (exist _ [] H) _ _ => absurd0 H
     | deep (exist _ [a] _) m r =>
         match viewL _ m with
-        | emptyL _ => consL a (digitToTree r)
+        | emptyL => consL a (digitToTree r)
         | consL b c => consL a (deep (nodeToDigit b) c r)
         end
     | deep (exist _ [a; b] _) m r => consL a (deep {[b]} m r)
@@ -130,12 +184,12 @@ Defined.
 Fixpoint viewR {A : Type} (t : FingerTree A) : ViewR A.
   refine (
     match t with
-    | empty _ => emptyR _
-    | single a => consR (empty _) a
+    | empty => emptyR
+    | single a => consR empty a
     | deep _ _ (exist _ [] H) => absurd0 H
     | deep l m (exist _ [a] _) =>
         match viewR _ m with
-        | emptyR _ => consR (digitToTree l) a
+        | emptyR => consR (digitToTree l) a
         | consR b c => consR (deep l b (nodeToDigit c)) a
         end
     | deep l m (exist _ [a; b] _) => consR (deep l m {[a]}) b
@@ -144,6 +198,44 @@ Fixpoint viewR {A : Type} (t : FingerTree A) : ViewR A.
     | deep l m (exist _ _ H) => absurd5 H
     end
   ); simpl in *; intuition.
+Defined.
+
+Definition semiDigitConcatTree {A : Type} (x : SemiDigit A)
+                                          (t : FingerTree A) : FingerTree A :=
+  match x with
+  | exist _ [] _ => t
+  | exist _ [a] _ => a <| t
+  | exist _ [a; b] _ => a <| b <| t
+  | exist _ [a; b; c] _ => a <| b <| c <| t
+  | exist _ [a; b; c; d] _ => a <| b <| c <| d <| t
+  | exist _ _ H => absurd5 H
+  end.
+
+Definition treeConcatSemiDigit {A : Type} (t : FingerTree A)
+                                          (x : SemiDigit A) : FingerTree A :=
+  match x with
+  | exist _ [] _ => t
+  | exist _ [a] _ => t |> a
+  | exist _ [a; b] _ => t |> a |> b
+  | exist _ [a; b; c] _ => t |> a |> b |> c
+  | exist _ [a; b; c; d] _ => t |> a |> b |> c |> d
+  | exist _ _ H => absurd5 H
+  end.
+
+Fixpoint concatRec {A : Type} (a : FingerTree A)
+                              (b : SemiDigit A)
+                              (c : FingerTree A) : FingerTree A :=
+  match a, c with
+  | empty, _ => semiDigitConcatTree b c
+  | single a, _ => a <| semiDigitConcatTree b c
+  | _, empty => treeConcatSemiDigit a b
+  | _, single c => treeConcatSemiDigit a b |> c
+  | deep l1 m1 r1, deep l2 m2 r2 =>
+      deep l1 (concatRec m1 (fromDigit (concatDigits r1 b l2)) m2) r2
+  end.
+
+Definition concat {A : Type} (t1 t2 : FingerTree A) : FingerTree A.
+  refine (concatRec t1 {[]} t2); simpl; omega.
 Defined.
 
 (** Abstract relation w.r.t. simple list. *)
@@ -155,14 +247,14 @@ Inductive AbsRelateNode : forall (A : Type), Node A -> list A -> Prop :=
 
 Inductive AbsRelateTree : forall (A : Type), FingerTree A -> list A -> Prop :=
 | abs_relate_empty : forall (A : Type),
-    AbsRelateTree (empty A) []
+    AbsRelateTree (@empty A) []
 | abs_relate_single : forall (A : Type) (a : A),
     AbsRelateTree (single a) [a]
 | abs_relate_deep : forall (A : Type) (l r : Digit A) (m : FingerTree (Node A))
                            (x : list (Node A)) (y : list (list A)),
     AbsRelateTree m x ->
     Forall2 (@AbsRelateNode A) x y ->
-    AbsRelateTree (deep l m r) (proj1_sig l ++ concat y ++ proj1_sig r).
+    AbsRelateTree (deep l m r) (proj1_sig l ++ List.concat y ++ proj1_sig r).
 
 Lemma abs_relate_tree_eq :
   forall (A : Type) (t : FingerTree A) l l',
@@ -183,6 +275,7 @@ Ltac break_match :=
   end; subst.
 
 Hint Rewrite <- app_assoc : app.
+Hint Rewrite app_nil_r : app.
 Hint Rewrite concat_app : app.
 
 Theorem cons_relate :
@@ -311,4 +404,78 @@ Proof.
       autorewrite with app using auto.
 Qed.
 
-(** TODO: append. *)
+Lemma semiDigitConcatTree_relate :
+  forall (A : Type) (t : FingerTree A) (x : SemiDigit A) (l : list A),
+    AbsRelateTree t l ->
+    AbsRelateTree (semiDigitConcatTree x t) (proj1_sig x ++ l).
+Proof.
+  intros.
+  destruct x as [x H1].
+  do 5 (destruct x as [| ?]; repeat apply cons_relate; auto).
+  simpl in H1; omega.
+Qed.
+
+Lemma treeConcatSemiDigit_relate :
+  forall (A : Type) (t : FingerTree A) (x : SemiDigit A) (l : list A),
+    AbsRelateTree t l ->
+    AbsRelateTree (treeConcatSemiDigit t x) (l ++ proj1_sig x).
+Proof.
+  intros.
+  destruct x as [x H1].
+  do 5 (destruct x as [| ?]; autorewrite with app; simpl;
+        eapply abs_relate_tree_eq; repeat apply snoc_relate; eauto;
+        autorewrite with app using auto).
+  simpl in H1; omega.
+Qed.
+
+Theorem nodeToList_Forall_relate :
+  forall (A : Type) (l : list (Node A)),
+    Forall2 (AbsRelateNode (A:=A)) l (map (nodeToList (A:=A)) l).
+Proof.
+  induction l; simpl; auto.
+  constructor; auto.
+  destruct a; simpl; constructor.
+Qed.
+
+Lemma concatRec_relate :
+  forall (A : Type) (t1 t2 : FingerTree A) (x : SemiDigit A) (l1 l2 : list A),
+    AbsRelateTree t1 l1 ->
+    AbsRelateTree t2 l2 ->
+    AbsRelateTree (concatRec t1 x t2) (l1 ++ proj1_sig x ++ l2).
+Proof.
+  induction t1; intros; simpl.
+  - inv_abs H.
+    apply semiDigitConcatTree_relate; auto.
+  - inv_abs H.
+    apply cons_relate. apply semiDigitConcatTree_relate; auto.
+  - destruct t2.
+    + inv_abs H0. autorewrite with app.
+      apply treeConcatSemiDigit_relate; auto.
+    + inv_abs H0.
+      eapply abs_relate_tree_eq.
+      apply snoc_relate; apply treeConcatSemiDigit_relate; eauto.
+      autorewrite with app using auto.
+    + inv_abs H; inv_abs H0.
+      eapply abs_relate_tree_eq. econstructor.
+      eapply IHt1; eauto.
+      apply Forall2_app; eauto.
+      apply Forall2_app; eauto.
+      apply nodeToList_Forall_relate.
+      destruct d0; destruct x; destruct d1.
+      do 5 (try (destruct x2));
+      do 6 (try (destruct x));
+      do 5 (try (destruct x3));
+      simpl in a; simpl in a0; simpl in a1; try omega; simpl;
+      autorewrite with app using auto.
+Qed.
+
+Lemma concat_relate :
+  forall (A : Type) (t1 t2 : FingerTree A) (l1 l2 : list A),
+    AbsRelateTree t1 l1 ->
+    AbsRelateTree t2 l2 ->
+    AbsRelateTree (concat t1 t2) (l1 ++ l2).
+Proof.
+  unfold concat; intros.
+  eapply abs_relate_tree_eq. apply concatRec_relate; eauto.
+  auto.
+Qed.
